iris_heap_lang/adequacy.v
@@ -1,4 +1,4 @@
-From iris.algebra Require Import auth.
+From iris.algebra Require Import lib.frac_auth numbers auth.
 From iris.proofmode Require Import tactics.
 From iris.program_logic Require Export weakestpre adequacy.
 From iris.heap_lang Require Import proofmode notation.
@@ -9,10 +9,12 @@ Class heapPreG Σ := HeapPreG {
   heap_preG_heap :> gen_heapPreG loc (option val) Σ;
   heap_preG_inv_heap :> inv_heapPreG loc (option val) Σ;
   heap_preG_proph :> proph_mapPreG proph_id (val * val) Σ;
+  heap_preG_credit_inG :> inG Σ (frac_authR natR);
 }.
 
 Definition heapΣ : gFunctors :=
-  #[invΣ; gen_heapΣ loc (option val); inv_heapΣ loc (option val); proph_mapΣ proph_id (val * val)].
+  #[invΣ; gen_heapΣ loc (option val); inv_heapΣ loc (option val); proph_mapΣ proph_id (val * val);
+    GFunctor (frac_authR natR)].
 Global Instance subG_heapPreG {Σ} : subG heapΣ Σ → heapPreG Σ.
 Proof. solve_inG. Qed.
 
@@ -20,12 +22,19 @@ Definition heap_adequacy Σ `{!heapPreG Σ} s e σ φ :
   (∀ `{!heapG Σ}, ⊢ inv_heap_inv -∗ WP e @ s; ⊤ {{ v, ⌜φ v⌝ }}) →
   adequate s e σ (λ v _, φ v).
 Proof.
-  intros Hwp; eapply (wp_adequacy _ _); iIntros (? κs) "".
+  intros Hwp; eapply (wp_adequacy' _ _); iIntros (? κs) "".
   iMod (gen_heap_init σ.(heap)) as (?) "[Hh _]".
   iMod (inv_heap_init loc (option val)) as (?) ">Hi".
   iMod (proph_map_init κs σ.(used_proph_id)) as (?) "Hp".
-  iModIntro. iExists
-    (λ σ κs, (gen_heap_interp σ.(heap) ∗ proph_map_interp κs σ.(used_proph_id))%I),
-    (λ _, True%I).
-  iFrame. iApply (Hwp (HeapG _ _ _ _ _)). done.
+  iMod (own_alloc (●F O ⋅ ◯F 0)) as (γ) "[Hγ Hγ']";
+    first by apply auth_both_valid_discrete.
+  iModIntro.
+  set (hG := (HeapG _ _ _ _ _ _ γ)).
+  iExists
+    (λ σ ns κs nt, (cred_interp ns ∗ gen_heap_interp σ.(heap) ∗ proph_map_interp κs σ.(used_proph_id))%I),
+    (λ _, True%I), _.
+  iFrame.
+  iSplitL "Hγ'".
+  { iExists 1%Qp. iFrame. }
+  iApply (Hwp (HeapG _ _ _ _ _ _ γ)). done.
 Qed.
