iris_heap_lang/total_adequacy.v
@@ -1,3 +1,4 @@
+From iris.algebra Require Import lib.frac_auth numbers auth.
 From iris.proofmode Require Import tactics.
 From iris.program_logic Require Export total_adequacy.
 From iris.heap_lang Require Export adequacy.
@@ -8,13 +9,19 @@ Definition heap_total Σ `{!heapPreG Σ} s e σ φ :
   (∀ `{!heapG Σ}, ⊢ inv_heap_inv -∗ WP e @ s; ⊤ [{ v, ⌜φ v⌝ }]) →
   sn erased_step ([e], σ).
 Proof.
-  intros Hwp; eapply (twp_total _ _); iIntros (?) "".
+  intros Hwp; eapply (twp_total' _ _); iIntros (?) "".
   iMod (gen_heap_init σ.(heap)) as (?) "[Hh _]".
   iMod (inv_heap_init loc (option val)) as (?) ">Hi".
   iMod (proph_map_init [] σ.(used_proph_id)) as (?) "Hp".
+  iMod (own_alloc (●F O ⋅ ◯F 0)) as (γ) "[Hγ Hγ']";
+    first by apply auth_both_valid_discrete.
   iModIntro.
+  set (hG := (HeapG _ _ _ _ _ _ γ)).
   iExists
-    (λ σ κs _, (gen_heap_interp σ.(heap) ∗ proph_map_interp κs σ.(used_proph_id))%I),
-    (λ _, True%I); iFrame.
-  iApply (Hwp (HeapG _ _ _ _ _)). done.
+    (λ σ ns κs _, (cred_interp ns ∗ gen_heap_interp σ.(heap) ∗ proph_map_interp κs σ.(used_proph_id))%I),
+    (λ _, True%I), _; iFrame.
+  iFrame.
+  iSplitL "Hγ'".
+  { iExists 1%Qp. iFrame. }
+  iApply (Hwp (HeapG _ _ _ _ _ _ _)). done.
 Qed.
